

## Information Matrix Equality

### Step 1

Define the score of the log likelihood as

$$s_i(\theta) \equiv \nabla_{\theta} l_i(\theta)' = \left[ \frac{\partial l_i}{\partial \theta_1}, \dots, \frac{\partial l_i}{\partial \theta_P} \right]'$$

We now first show that

$$E[s_i(\theta)|x_i] = 0$$

This is simply to apply the definition of conditional expectation operator and the fact that  $l_i(\theta) = \log f(y_i|x_i; \theta)$

$$\begin{aligned} E[s_i(\theta)|x_i] &= \int s_i(\theta) f(y|x_i; \theta) \nu(dy) \\ &= \int \nabla_{\theta} f(y|x_i; \theta) \nu(dy) \\ &= \nabla_{\theta} \int f(y|x_i; \theta) \nu(dy) \\ &= 0 \end{aligned}$$

### Step 2

Now we are equipped to show the conditional information matrix equality. Use the fact that  $E[s_i(\theta)|x_i] = 0$  and take derivative on both side.

$$\begin{aligned} \nabla_{\theta} E[s_i(\theta)|x_i] &\equiv \nabla_{\theta} \left[ \int s_i(\theta) f(y|x_i; \theta) \nu(dy) \right] \\ &= \int \nabla_{\theta} [s_i(\theta) f(y|x_i; \theta)] \nu(dy) = 0 \end{aligned}$$

Recall that  $H_i(\theta) \equiv \nabla_{\theta} s_i(\theta) = \nabla_{\theta}^2 l_i(\theta)$ . Thus

$$\nabla_{\theta} [s_i(\theta) f(y|x_i; \theta)] = H_i(\theta) f(y|x_i; \theta) + s_i(\theta) s_i(\theta)' f(y|x_i; \theta)$$

So we have

$$\begin{aligned} \int [H_i(\theta) + s_i(\theta) s_i(\theta)'] f(y|x_i; \theta) \nu(dy) &= 0 \\ -E[H_i(\theta)|x_i] &= E[s_i(\theta) s_i(\theta)'|x_i] \end{aligned}$$

### Step 3

Now we evaluate both conditional expectations at  $\theta_0$ , we reach the conditional information matrix equality

$$-E[H_i(\theta_0)|x_i] = E[s_i(\theta_0)s_i(\theta_0)'|x_i]$$

Use the law of iterated expectations (with respect to the distribution of  $x_i$ ), we have  $A_0 = B_0$ .